src/tree/layer1/UnorderedSet.dfy
@@ -1,0 +1,307 @@
+include "../../../src/Utils.dfy"
+
+
+trait UnorderedSetIterator {
+  function Parent(): UnorderedSet
+    reads this
+
+  predicate Valid()
+    reads this, Parent(), Parent().Repr()
+
+  function Model(): (set<int>,int) //already traversed elements+ maybe elem
+    reads this, Parent(), Parent().Repr()
+    requires Valid()
+    requires Parent().Valid() 
+    ensures {} <=Model().0 <=Parent().Model()
+    ensures Model().0 < Parent().Model() ==> 
+             Model().1 in  Parent().Model() && Model().1 !in Model().0 
+
+  function method HasNext(): bool
+    reads this, Parent(), Parent().Repr()
+    requires Valid()
+    requires Parent().Valid()
+    ensures HasNext() ==> Model().0 < Parent().Model() && |Model().0| < |Parent().Model()|
+    ensures !HasNext() ==> Model().0 == Parent().Model() && |Model().0| == |Parent().Model()|
+  /*function method HasPrev(): bool
+    reads this, Parent(), Parent().Repr()
+    requires Valid()
+    requires Parent().Valid()
+    ensures HasPrev() <==> Model().0 != {}*/
+
+  method Next() returns (x: int)
+    modifies this
+    requires Valid()
+    requires Parent().Valid()
+    requires HasNext()
+    requires allocated(Parent())
+    requires forall it | it in Parent().Repr() :: allocated(it)
+    ensures Parent().Valid()
+    ensures Valid()
+    ensures old(Parent()) == Parent()
+    ensures old(Parent().Model()) == Parent().Model()
+
+    ensures forall x {:trigger x in Parent().Repr(), x in old(Parent().Repr())} | x in Parent().Repr() - old(Parent().Repr()) :: fresh(x)
+    ensures fresh(Parent().Repr()-old(Parent().Repr()))
+    ensures forall x | x in Parent().Repr() :: allocated(x)
+
+    ensures Parent().Iterators() == old(Parent().Iterators())
+
+    ensures x==old(Model().1) && {old(Model().1)}+old(Model().0)==Model().0 //> old(Model().0)
+    ensures HasNext() ==> Model().1 in Parent().Model() && Model().1 !in Model().0
+    
+    ensures forall it | it in Parent().Iterators() && old(it.Valid()) ::
+      it.Valid() && (it != this ==> it.Model() == old(it.Model()))
+
+
+  function method Peek(): int
+    reads this, Parent(), Parent().Repr()
+    requires Valid()
+    requires Parent().Valid()
+    requires HasNext()
+    ensures Peek() == Model().1
+
+  method Copy() returns (it: UnorderedSetIterator)
+    modifies Parent(), Parent().Repr()
+    requires Valid()
+    requires Parent().Valid()
+    requires allocated(Parent())
+    requires forall it | it in Parent().Iterators() :: allocated(it)
+    ensures fresh(it)
+    ensures Valid()
+    ensures Parent() == old(Parent())
+    ensures Parent().Valid()
+    ensures Parent().Model() == old(Parent().Model())
+
+    ensures forall x {:trigger x in Parent().Repr(), x in old(Parent().Repr())} | x in Parent().Repr() - old(Parent().Repr()) :: fresh(x)
+    ensures fresh(Parent().Repr()-old(Parent().Repr()))
+    ensures forall x | x in Parent().Repr() :: allocated(x)
+    
+    ensures it.Valid()
+    ensures Parent().Iterators() == {it} + old(Parent().Iterators())
+    ensures Parent() == it.Parent()
+    ensures Model() == it.Model()
+    ensures forall it | it in old(Parent().Iterators()) && old(it.Valid()) ::
+      it.Valid() && it.Model() == old(it.Model())
+
+  
+}
+
+trait UnorderedSet {
+  function ReprDepth(): nat
+    ensures ReprDepth() > 0
+
+  function ReprFamily(n: nat): set<object>
+    decreases n
+    requires n <= ReprDepth()
+    ensures n > 0 ==> ReprFamily(n) >= ReprFamily(n-1)
+    reads this, if n == 0 then {} else ReprFamily(n-1)
+
+  function Repr(): set<object>
+    reads this, ReprFamily(ReprDepth()-1)
+  {
+    ReprFamily(ReprDepth())
+  }
+
+  lemma UselessLemma()
+    ensures Repr() == ReprFamily(ReprDepth());
+
+  predicate Valid()
+    reads this, Repr()
+
+  function Model(): set<int>
+    reads this, Repr()
+    requires Valid()
+
+  function method Empty(): bool
+    reads this, Repr()
+    requires Valid()
+    ensures Empty() <==> Model() == {}
+
+  function method Size(): nat
+    reads this, Repr()
+    requires Valid()
+    ensures Size() == |Model()|
+
+  function Iterators(): set<UnorderedSetIterator>
+    reads this, Repr()
+    requires Valid()
+    ensures forall it | it in Iterators() :: it in Repr() && it.Parent() == this
+
+method First() returns (it: UnorderedSetIterator)
+    modifies this, Repr()
+    requires Valid()
+    requires forall x | x in Repr() :: allocated(x)
+    ensures Valid()
+    ensures Model() == old(Model())
+
+    ensures forall x {:trigger x in Repr(), x in old(Repr())} | x in Repr() - old(Repr()) :: fresh(x)
+    ensures fresh(Repr()-old(Repr()))
+    ensures forall x | x in Repr() :: allocated(x)
+
+    ensures fresh(it)
+    ensures Iterators() == {it} + old(Iterators())
+    ensures it.Valid()
+    ensures it.Model().0=={} && (Model()!={}==> it.Model().1 in Model())
+    ensures it.Parent() == this
+    ensures forall it | it in old(Iterators()) && old(it.Valid()) ::
+      it.Valid() && it.Model() == old(it.Model())
+
+ 
+
+  method contains(x:int) returns (b:bool)
+    requires Valid()
+    ensures Valid() && b == (x in Model())
+
+  method add(x:int)
+    modifies this,Repr()
+    requires Valid()
+    requires forall x | x in Repr() :: allocated(x)
+    ensures Valid()
+    ensures Model() == old(Model()) + {x} 
+
+    ensures forall x {:trigger x in Repr(), x in old(Repr())} | x in Repr() - old(Repr()) :: fresh(x)
+    ensures fresh(Repr()-old(Repr()))
+    ensures forall x | x in Repr() :: allocated(x)
+   
+    ensures Iterators() == old(Iterators())
+
+
+
+  method remove(x:int) 
+    modifies this,Repr()
+    requires Valid()
+    requires forall x | x in Repr() :: allocated(x)
+    ensures Valid()
+    ensures Model()== old(Model()) - {x} 
+
+    ensures forall x {:trigger x in Repr(), x in old(Repr())} | x in Repr() - old(Repr()) :: fresh(x)
+    ensures fresh(Repr()-old(Repr()))
+    ensures forall x | x in Repr() :: allocated(x)
+
+    ensures Iterators() == old(Iterators())
+
+
+  method find(x:int) returns (newt:UnorderedSetIterator)
+    requires Valid()
+    requires forall x | x in Repr() :: allocated(x)
+    ensures Valid() 
+    ensures fresh(newt) 
+    ensures newt.Valid() && newt.Parent()==this
+    ensures x in Model() ==> newt.Model().0=={} && newt.Model().1==x
+    ensures x !in Model() ==> newt.Model().0==Model()
+
+    ensures forall x {:trigger x in Repr(), x in old(Repr())} | x in Repr() - old(Repr()) :: fresh(x)
+    ensures fresh(Repr()-old(Repr()))
+    ensures forall x | x in Repr() :: allocated(x)
+    ensures Iterators() == {newt}+old(Iterators())
+
+  method insert(mid: UnorderedSetIterator, x: int) returns (newt:UnorderedSetIterator)
+    modifies this, Repr()
+    requires Valid()
+    requires mid.Valid() 
+    requires mid.Parent() == this
+    requires mid in Iterators()
+    requires forall x | x in Repr() :: allocated(x)
+    ensures Valid()
+    ensures Model() == old(Model()) + {x}
+
+    ensures forall x {:trigger x in Repr(), x in old(Repr())} | x in Repr() - old(Repr()) :: fresh(x)
+    ensures fresh(Repr()-old(Repr()))
+    ensures forall x | x in Repr() :: allocated(x)
+
+    ensures fresh(newt)
+    ensures Iterators() == {newt}+old(Iterators())
+    ensures newt.Valid() && newt.Parent()==this && newt.HasNext()
+    ensures newt.Model().0==(old(mid.Model().0)-{x}) && newt.Model().1==x //??DUDA
+    //points either to the inserted elemento or to the already existing one
+ 
+
+
+  method erase(mid:UnorderedSetIterator) returns (next: UnorderedSetIterator)
+    modifies this, Repr()
+    requires Valid()
+    requires mid.Valid()
+    requires mid.Parent() == this
+    requires mid.HasNext()
+    requires mid in Iterators()
+    requires forall x | x in Repr() :: allocated(x)
+    ensures Valid()
+    ensures Model()== old(Model())-{old(mid.Model().1)}
+    
+    ensures fresh(next)
+    ensures Iterators() == {next}+old(Iterators())
+    ensures next.Valid() && next.Parent()==this 
+    ensures next.Model().0==old(mid.Model().0) && 
+       (Model()!={} ==> next.Model().1 in Model() && next.Model().1 !in next.Model().0)
+}
+
+
+
+method {:verify true} try(s:UnorderedSet)
+modifies s, s.Repr()
+requires s.Valid() && s.Empty()
+requires forall x | x in s.Repr() :: allocated(x)
+ensures s.Valid()
+ensures forall x {:trigger x in s.Repr(), x in old(s.Repr())} | x in s.Repr() - old(s.Repr()) :: fresh(x)
+ensures fresh(s.Repr()-old(s.Repr()))
+ensures forall x | x in s.Repr() :: allocated(x)
+{
+ s.add(3);
+ s.add(4);
+ assert 3 in s.Model();
+ assert 4 in s.Model();
+ assert (set x | x in s.Model()) == {3,4};
+ s.add(4);
+ assert (set x | x in s.Model()) == {3,4};
+ s.remove(2);
+  assert (set x | x in s.Model()) == {3,4};
+ s.remove(3);
+  assert (set x | x in s.Model()) == {4};
+ s.remove(4);
+   assert (set x | x in s.Model()) == {};
+ s.add(2); s.add(7); s.add(0); s.add(1);s.add(10);
+
+ var b:=s.contains(10);
+ assert b;
+
+   var s1:set<int>;
+   var s2:set<int>;
+   s1:={1,2,4};
+   s2:={0,1,2,3,4,8};
+   assert s1<=s2;
+   assert |s1|<=|s2|;
+
+
+ var it:=s.First(); var cont:=0; /*ghost var omodel:=s.Model();
+ assert |it.Model().0|<=|s.Model()|;
+assert !it.HasNext() ==> |it.Model().0|==|s.Model()|;
+assert |s.Model()|-|it.Model().0|>=0;*/
+  while (it.HasNext())
+     decreases |s.Model()|-|it.Model().0|
+     invariant it.Valid() && it.Parent()==s  
+     invariant s.Valid()
+     invariant  forall x {:trigger x in s.Repr(), x in old(s.Repr())} | x in s.Repr() - old(s.Repr()) :: fresh(x)
+     invariant fresh(s.Repr()-old(s.Repr()))
+     invariant forall x | x in s.Repr() :: allocated(x)
+    {
+     var aux:=it.Next();
+     if (aux%2==0) {cont:=cont+1;} 
+    } 
+  var it2:=s.find(2);
+  assert it2.Model().1==2;
+  it2:=s.find(7); 
+  assert it.Model().1==7;  
+  var aux:=it.Next();
+  assert aux==7;assert it.Model().0=={2,7,1,0,10};
+  
+  var it3:=s.find(7);
+  it3:=s.insert(it3,5);
+  assert it3.Model().1==5;
+  it3:=s.insert(it3,12);
+  assert it3.Model().1==12;
+  assert it3.Model().0=={};
+   aux:=it3.Next();
+   assert 12 in it3.Model().0;
+   aux:=it3.Next();
+   assert 12 in it3.Model().0;
+}
